Language_Components/Imp_Ctl/Imp_Ctl.thy
@@ -1,0 +1,91 @@
+theory Imp_Ctl
+imports "../../Syntax/Gensyn" "../../Syntax/Gensyn_Descend" "../../Mergeable/Mergeable"
+        "../../Mergeable/Mergeable_Instances"
+        "../../Lifter/Lifter" "../../Lifter/Lifter_Instances"
+        "../../Lifter/Auto_Lifter" "../../Lifter/Auto_Lifter_Proofs" 
+        "../../Semantics/Semantics" "../../Composition/Dominant"
+        "../Utils"
+        "Cond"
+begin
+
+(*
+ * Implementation of standard imperative-language control structures (If and While).
+ * These are based off the idealized language IMP (see e.g. _Software Foundations_ vol. 1,, "Imp")
+ * and lack constructs such as break and continue. However, the framework is flexible enough
+ * to permit description of such constructs and even write Hoare rules for them
+ * (for an example of how this might work, see Appel and Blazy,
+ * "Separation Logic for Small-Step Cminor")
+ *)
+
+(* SWhileC is a while loop in which the condition check is reduced to check of whether
+ * a fixed flag (a boolean shared between the cond language state and the
+ * imp language state) is true. This makes the Hoare rule somewhat simpler to express.
+ *)
+datatype syn' =
+  Sif
+  | Sskip
+  | SwhileC
+
+type_synonym 'x imp_state' = "'x gensyn list * bool"
+
+type_synonym 'x state' = "'x gensyn list * bool * int"
+
+definition imp_ctl_sem :: "syn' \<Rightarrow> 'x imp_state' \<Rightarrow> 'x imp_state'" where
+"imp_ctl_sem x st =
+  (case st of
+    ([], b) \<Rightarrow> ([], b)
+    | ((G z l)#t, b) \<Rightarrow>
+      ((case x of
+        Sskip \<Rightarrow> t
+        | Sif \<Rightarrow>
+        (case l of
+          [body] \<Rightarrow> (if b then body#t else t)
+          | [cond, body] \<Rightarrow> cond# ((G z [body])#t)
+          | _ \<Rightarrow> [] \<comment>\<open> error \<close>)
+        | SwhileC \<Rightarrow>
+        (case l of [body] \<Rightarrow> (if b then body # (G z [body]) # t else t)
+         | _ \<Rightarrow> [] \<comment>\<open> error \<close>))
+      , b))"
+
+
+type_synonym ('s, 'x) state = 
+  "('s, (bool md_triv option md_prio * int md_triv option md_prio * 'x)) control"
+
+type_synonym ('s) cstate = 
+  "('s, unit option) state"
+
+
+
+definition imp_prio :: "(syn' \<Rightarrow> nat)" where
+"imp_prio x =
+(case x of
+    Sskip \<Rightarrow> 0
+    | _ \<Rightarrow> 2)"
+
+
+definition imp_sem_lifting_gen :: "(syn', 'x imp_state', 
+                                   ('x, _ ) state) lifting" where
+"imp_sem_lifting_gen = 
+ (schem_lift (SP NA NB)
+             (SP (SPRC imp_prio (SO NA)) (SP NX (SP (SPRK (SO NB)) NX))))"
+
+
+definition imp_sem_l_gen :: "('s \<Rightarrow> syn') \<Rightarrow> 's \<Rightarrow> ('x, 'z :: Mergeableb) state \<Rightarrow> ('x, 'z) state" where
+"imp_sem_l_gen lfts =
+  lift_map_s lfts
+    imp_sem_lifting_gen
+  imp_ctl_sem"
+
+
+definition get_cond :: 
+"bool md_triv option md_prio * 
+  int md_triv option md_prio * 
+  (_ :: Pordb) \<Rightarrow> bool option" where
+"get_cond st = 
+  (case st of
+    (b, _, _) \<Rightarrow> 
+    (case b of
+      (mdp _ (Some (mdt b'))) \<Rightarrow> Some b'
+      | _ \<Rightarrow> None))"
+
+end
