Language_Components/Imp_Ctl/Imp_Ctl_Hoare.thy
@@ -1,0 +1,501 @@
+theory Imp_Ctl_Hoare
+  imports Imp_Ctl "../../Hoare/Hoare"  "../../Hoare/Hoare_Indexed"
+  "../../Hoare/Hoare_Indexed_Sound"
+begin
+
+(* Implementation of Hoare rules for WHILE and IF.
+ * Provides an interesting example of using the step-count-indexed version of Hoare
+ * logic to prove a theorem not easily provable without that abstraction
+ * (this was what motivated the development of that abstraction).
+ *)
+
+(* This if rule looks a bit different from the traditional one;
+ * this is mostly because evaluation of the condition (cond) may have
+ * side effects. *)
+lemma HIf :
+  assumes H0 : "gs = pcomps fs"
+  assumes HF : "f = imp_sem_l_gen lfts"
+  assumes Hpres : "sups_pres (set fs)"
+  assumes Hnemp : "g \<in> set fs"
+  assumes Hdom : "(f \<downharpoonleft> (set fs) Sif')"
+  assumes Hsyn : "lfts Sif' = Sif"
+  assumes P1_valid : "\<And> st.  P1 st \<Longrightarrow> get_cond st \<noteq> None"
+  assumes P2_valid : "\<And> st . P2 st \<Longrightarrow> get_cond st \<noteq> None"
+
+  assumes Hcond : "|gs| {- P1 -} [cond] {- P2 -}"
+  assumes Htrue : "|gs| {- (\<lambda> st . P2 st \<and> get_cond st = Some True) -} [body]
+                        {- P3 -}"
+  assumes Hfalse : "|gs| {- (\<lambda> st . P2 st \<and> get_cond st = Some False) -} [] {-P3-}"
+  shows "|gs| {- P1 -} [G Sif' [cond, body]] {- P3 -}"
+proof
+  fix c'
+  assume Guard : "|gs| {P3} c'"
+
+  have Gtrue : "|gs| {(\<lambda>st. P2 st \<and> get_cond st = Some True)} ([body] @ c')"
+    using HTE[OF Htrue Guard] by auto
+
+  have Gfalse : "|gs| {(\<lambda>st. P2 st \<and> get_cond st = Some False)} ([] @ c')"
+    using HTE[OF Hfalse Guard] by auto
+
+  show "|gs| {P1} ([G Sif' [cond, body]] @ c')"
+  proof
+    fix m :: "('a, 'b) state"
+
+    assume M : "P1 (payload m)"
+    assume CM : "cont m = Inl ([G Sif' [cond, body]] @ c')"
+
+    show "(safe gs m)"
+    proof(cases "(sem_step gs m)")
+      case (Inr bad)
+
+      then have False using CM H0
+        by(auto simp add: sem_step_def)
+
+      then show ?thesis by auto
+    next
+      case (Inl m')
+
+      have F_eq : "sem_step f m = Inl m'"
+        using sym[OF dominant_pcomps[OF Hpres Hnemp Hdom]] CM Inl H0
+        by(simp add: sem_step_def)
+
+      have CM' : "cont m' = Inl ([cond] @ ([ G Sif' [body]] @ c'))" 
+        using CM Hsyn F_eq unfolding HF
+        by(cases m; auto simp add: cont_def sem_step_def imp_sem_l_gen_def imp_ctl_sem_def imp_sem_lifting_gen_def
+           schem_lift_defs 
+          merge_l_def fst_l_def snd_l_def prio_l_def triv_l_def option_l_def
+          split: md_prio.splits md_triv.splits option.splits)
+
+      have M'_valid : "\<And> p . fst (payload m) \<noteq> mdp p None" using P1_valid[OF M]
+        by(auto simp add: get_cond_def split:prod.splits)
+
+      have Sm' : "payload m = payload m'"
+        using CM Hsyn F_eq M'_valid  unfolding HF
+        by(cases m; auto simp add: cont_def sem_step_def imp_sem_l_gen_def imp_ctl_sem_def imp_sem_lifting_gen_def
+           schem_lift_defs 
+          merge_l_def fst_l_def snd_l_def prio_l_def triv_l_def option_l_def LNew_def
+          split: md_prio.splits md_triv.splits option.splits)
+
+      hence P1sm' : "P1 (payload m')" using M unfolding Sm' by auto
+
+      (* step to the end of cond. *)
+
+      have Sub : "|gs| {P2} ([G Sif' [body]] @ c')"
+      proof
+        fix mp2 :: "('a, 'b) state"
+
+        assume MP2 : "P2 (payload mp2)"
+
+        assume Cont2 : "cont mp2 = Inl ([G Sif' [body]] @ c')"
+
+        show "safe gs mp2"
+        proof(cases "get_cond (payload mp2)")
+          case None
+
+          then have False using P2_valid[OF MP2]
+            by(auto simp add: get_cond_def split: prod.splits md_prio.splits md_triv.splits option.splits)
+          then show ?thesis by auto
+
+        next
+          case Some' : (Some cnd)
+          then show ?thesis 
+          proof(cases "sem_step gs mp2")
+            case (Inr bad)
+
+            then have False using Cont2 H0
+              by(auto simp add: sem_step_def)
+
+            then show ?thesis by auto
+
+          next
+            case (Inl mp2')
+
+            have F_eq' : "sem_step f mp2 = Inl mp2'"
+              using sym[OF dominant_pcomps[OF Hpres Hnemp Hdom]] Cont2 Inl H0
+              by(simp add: sem_step_def)
+
+            have Mp2'_p2 : "P2 (payload mp2')"
+              using Cont2 Hsyn H0 MP2 F_eq' P2_valid[OF MP2] Some' unfolding HF
+              by(cases mp2; 
+                  auto simp add: cont_def sem_step_def imp_sem_l_gen_def imp_ctl_sem_def imp_sem_lifting_gen_def
+                  schem_lift_defs 
+                  merge_l_def fst_l_def snd_l_def prio_l_def triv_l_def option_l_def LNew_def
+                  get_cond_def
+                  split: md_prio.splits md_triv.splits option.splits)
+
+            show ?thesis
+            proof(cases cnd)
+              case True
+        
+              have Mp2'_cond : "get_cond (payload mp2') = Some True" 
+                using Cont2 Hsyn H0 MP2 F_eq' P2_valid[OF MP2] True Some' unfolding HF
+                by(cases mp2; 
+                    auto simp add: cont_def sem_step_def imp_sem_l_gen_def imp_ctl_sem_def imp_sem_lifting_gen_def
+                    schem_lift_defs 
+                    merge_l_def fst_l_def snd_l_def prio_l_def triv_l_def option_l_def LNew_def
+                    get_cond_def
+                    split: md_prio.splits md_triv.splits option.splits)
+
+              have Mp2'_p2_true :  "P2 (payload mp2') \<and> get_cond (payload mp2') = Some True"
+                using Mp2'_p2 Mp2'_cond
+                by auto
+
+              have Mp2'_cont : "cont mp2' = Inl ([body] @ c')"
+                using Cont2 Hsyn H0 MP2 F_eq' P2_valid[OF MP2] True Some' unfolding HF
+                by(cases mp2; cases mp2'; 
+                    auto simp add: cont_def sem_step_def imp_sem_l_gen_def imp_ctl_sem_def imp_sem_lifting_gen_def
+                    schem_lift_defs 
+                    merge_l_def fst_l_def snd_l_def prio_l_def triv_l_def option_l_def LNew_def
+                    get_cond_def
+                    split: md_prio.splits md_triv.splits option.splits)
+
+              have Mp2'_safe : "safe gs mp2'"
+                using guardedD[OF Gtrue Mp2'_p2_true Mp2'_cont] by auto
+
+              show ?thesis
+              proof
+                fix mz
+                assume Exec : "sem_exec_p gs mp2 mz"
+
+                show "imm_safe gs mz" using Exec unfolding sem_exec_p_def
+                proof(cases rule: rtranclp.cases)
+                  case rtrancl_refl
+
+                  then have "(\<exists>m'. sem_step gs mz = Inl m')"
+                    using Inl unfolding imm_safe_def sem_step_p_eq
+                    by(cases mp2'; auto)
+
+                  then show ?thesis unfolding imm_safe_def sem_step_p_eq by auto
+                next
+                  case (rtrancl_into_rtrancl b)
+
+                  have Step : "sem_step_p gs mp2 mp2'" using Inl
+                    unfolding sem_step_p_eq
+                    by auto
+        
+                  have Exec_final : "sem_exec_p gs mp2' mz"
+                    using rtranclp_bisect1
+                      [OF sem_step_determ rtrancl_into_rtrancl(1)
+                          Step rtrancl_into_rtrancl(2)]
+                    unfolding sem_exec_p_def
+                    by auto
+        
+                  show ?thesis using safeD[OF Mp2'_safe Exec_final] by auto 
+                qed
+              qed
+
+            next
+              case False
+
+              have Mp2'_cond : "get_cond (payload mp2') = Some False" 
+                using Cont2 Hsyn H0 MP2 F_eq' P2_valid[OF MP2] False Some' unfolding HF
+                by(cases mp2; 
+                    auto simp add: cont_def sem_step_def imp_sem_l_gen_def imp_ctl_sem_def imp_sem_lifting_gen_def
+                    schem_lift_defs 
+                    merge_l_def fst_l_def snd_l_def prio_l_def triv_l_def option_l_def LNew_def
+                    get_cond_def
+                    split: md_prio.splits md_triv.splits option.splits)
+
+              have Mp2'_p2_false :  "P2 (payload mp2') \<and> get_cond (payload mp2') = Some False"
+                using Mp2'_p2 Mp2'_cond
+                by auto
+
+              have Mp2'_cont : "cont mp2' = Inl ([] @ c')"
+                using Cont2 Hsyn H0 MP2 F_eq' P2_valid[OF MP2] False Some' unfolding HF
+                by(cases mp2; 
+                    auto simp add: cont_def sem_step_def imp_sem_l_gen_def imp_ctl_sem_def imp_sem_lifting_gen_def
+                    schem_lift_defs 
+                    merge_l_def fst_l_def snd_l_def prio_l_def triv_l_def option_l_def LNew_def
+                    get_cond_def
+                    split: md_prio.splits md_triv.splits option.splits)
+
+              have Mp2'_safe : "safe gs mp2'"
+                using guardedD[OF Gfalse Mp2'_p2_false Mp2'_cont] by auto
+
+              show ?thesis
+              proof
+                fix mz
+                assume Exec : "sem_exec_p gs mp2 mz"
+
+                show "imm_safe gs mz" using Exec unfolding sem_exec_p_def
+                proof(cases rule: rtranclp.cases)
+                  case rtrancl_refl
+
+                  then have "(\<exists>m'. sem_step gs mz = Inl m')"
+                    using Inl unfolding imm_safe_def sem_step_p_eq
+                    by(cases mp2'; auto)
+
+                  then show ?thesis unfolding imm_safe_def sem_step_p_eq by auto
+                next
+                  case (rtrancl_into_rtrancl b)
+
+                  have Step : "sem_step_p gs mp2 mp2'" using Inl
+                    unfolding sem_step_p_eq
+                    by auto
+        
+                  have Exec_final : "sem_exec_p gs mp2' mz"
+                    using rtranclp_bisect1
+                      [OF sem_step_determ rtrancl_into_rtrancl(1)
+                          Step rtrancl_into_rtrancl(2)]
+                    unfolding sem_exec_p_def
+                    by auto
+        
+                  show ?thesis using safeD[OF Mp2'_safe Exec_final] by auto 
+                qed
+              qed
+            qed
+          qed
+        qed
+      qed
+
+      have Guard' : "|gs| {P1} ([cond] @ ([G Sif' [body]] @ c'))"
+        using HTE[OF Hcond Sub] by auto
+
+      have Safe' : "safe gs m'" using guardedD[OF Guard' P1sm' CM'] by auto
+
+      show "safe gs m"
+      proof
+        fix mz
+
+        assume Z: "sem_exec_p gs m mz"
+
+        then show "imm_safe gs mz" unfolding sem_exec_p_def
+        proof(cases rule: rtranclp.cases)
+          case rtrancl_refl
+
+          then have "(\<exists>m'. sem_step gs mz = Inl m')"
+            using Inl unfolding imm_safe_def sem_step_p_eq
+            by(cases m'; auto)
+
+          then show ?thesis using Inl unfolding imm_safe_def sem_step_p_eq
+            by(auto)
+        next
+          case (rtrancl_into_rtrancl b)
+
+          have Step : "sem_step_p gs m m'" using Inl
+            unfolding sem_step_p_eq
+            by auto
+
+          have Exec_final : "sem_exec_p gs m' mz"
+            using rtranclp_bisect1
+              [OF sem_step_determ rtrancl_into_rtrancl(1)
+                  Step rtrancl_into_rtrancl(2)]
+            unfolding sem_exec_p_def
+            by auto
+
+          show ?thesis using safeD[OF Safe' Exec_final] by auto
+        qed
+      qed
+    qed
+  qed
+qed
+
+(* Some auxiliary definitions for proving the while rule *)
+lemma HWhileC_idx :
+  assumes H0 : "gs = pcomps fs"
+  assumes HF : "f = imp_sem_l_gen lfts"
+  assumes Hpres : "sups_pres (set fs)"
+  assumes Hnemp : "g \<in> set fs"
+  assumes Hdom : "(f \<downharpoonleft> (set fs) SwhileC')"
+  assumes Hsyn : "lfts SwhileC' = SwhileC"
+  assumes PX_valid : "\<And> st.  PX st \<Longrightarrow> get_cond st \<noteq> None"
+  assumes Htrue : "\<And> nb2 . \<exists> nb1' . |#gs#| {#- PX, (nb1' + nb2) -#} [body] {#- PX, nb2 -#}"
+  assumes NLs : "nl1 \<le> nl2"
+  shows "|#gs#| {#- PX, nl1  -#} [G SwhileC' [body]] {#- (\<lambda> st . PX st \<and> get_cond st = Some False), nl2 -#}"
+proof
+  fix c'
+
+  assume Guard : "|#gs#| {#(\<lambda>st. PX st \<and> get_cond st = Some False), nl2#} c'"
+
+  show "|#gs#| {#PX, nl1#} ([G SwhileC' [body]] @ c')" 
+    using Guard NLs
+  proof(induction nl2 arbitrary: nl1 c')
+    case 0
+    show ?case
+    proof
+      fix m :: "('a, 'b) state"
+      assume Hm : " PX (payload m)"
+
+      have Nl1_0 : "nl1 = 0" using 0 by auto
+
+      assume Hcontm : "cont m = Inl ([G SwhileC' [body]] @ c')" 
+
+
+      have Conc' : "sem_exec_c_p gs m 0 m \<and> cont m = Inl ((G SwhileC' [body]) # c')"
+        using Hcontm Excp_0[of gs m] by auto
+
+      show "safe_for gs m nl1" 
+        using Conc'
+        unfolding Nl1_0 safe_for_def
+        by blast
+    qed
+  next
+    case (Suc nl2')
+    show ?case 
+    proof
+      fix m :: "('a, 'b) state"
+      assume Hm : "PX (payload m)" 
+
+      assume Hcontm : "cont m = Inl ([G SwhileC' [body]] @ c')" 
+      show  "safe_for gs m nl1" 
+
+      proof(cases "(sem_step gs m)")
+        case (Inr bad)
+  
+        then have False using Hcontm H0
+          by(auto simp add: sem_step_def)
+  
+        then show ?thesis by auto
+      next
+        case (Inl m')
+
+        have F_eq : "sem_step f m = Inl m'"
+          using sym[OF dominant_pcomps[OF Hpres Hnemp Hdom]] Hcontm Inl H0
+          by(simp add: sem_step_def)
+  
+        have M_P1 : "PX (payload m)" using Hm Hcontm by auto
+  
+        have M'_valid : "\<And> p . fst (payload m) \<noteq> mdp p None" using PX_valid[OF M_P1]
+          by(auto simp add: get_cond_def split:prod.splits)
+  
+        have Sm' : "payload m = payload m'"
+          using Hcontm Hsyn F_eq M'_valid  unfolding HF
+          by(cases m; auto simp add: cont_def sem_step_def imp_sem_l_gen_def imp_ctl_sem_def imp_sem_lifting_gen_def
+             schem_lift_defs 
+            merge_l_def fst_l_def snd_l_def prio_l_def triv_l_def option_l_def LNew_def
+            split: md_prio.splits md_triv.splits option.splits)
+  
+        have M' : "PX (payload m')" using Sm' M_P1 by auto
+
+        show "safe_for gs m nl1"
+        proof(cases "get_cond (payload m)")
+          case None
+  
+          then have False using PX_valid[OF M_P1]
+            by(auto simp add: get_cond_def split: prod.splits md_prio.splits md_triv.splits option.splits)
+          then show ?thesis by auto
+  
+        next
+          case Some' : (Some cnd)
+
+          have Helper : "|#gs#| {#(\<lambda> st . PX st \<and> get_cond st = Some False), nl2'#} c'"
+          proof
+            fix ml :: "('a, 'b) state"
+            assume Hpay : "PX (payload ml) \<and> get_cond (payload ml) = Some False"
+
+            assume Hcont : "cont ml = Inl c'"
+
+            have Conc' : "safe_for gs ml (Suc nl2')"
+              using guardediD[OF Suc.prems(1) Hpay Hcont]
+              by auto
+
+            show "safe_for gs ml nl2'"
+              using safe_for_weaken[OF Conc', of nl2'] by auto
+          qed
+
+          show ?thesis
+          proof(cases cnd)
+            case True
+
+            have M'_cont : "cont m' = Inl ([body, G SwhileC' [body]] @ c')"
+                using Hsyn H0 M' F_eq True Some' Hcontm  unfolding HF
+                by(cases m; auto simp add: cont_def sem_step_def imp_sem_l_gen_def imp_ctl_sem_def imp_sem_lifting_gen_def
+                  schem_lift_defs 
+                  merge_l_def fst_l_def snd_l_def prio_l_def triv_l_def option_l_def LNew_def
+                  get_cond_def
+                  split: md_prio.splits md_triv.splits option.splits)
+
+            have G1 : "|#gs#| {#PX, nl2'#} ([G SwhileC' [body]] @ c')"
+              using Suc.IH[OF Helper] by auto
+
+            hence G1' :  "|#gs#| {#PX, (Suc nl2' - 1)#} ([G SwhileC' [body]] @ c')"
+              using Suc.IH[OF Helper] by auto
+
+            obtain nb where NB : "|#gs#| {#-PX, (nb + nl2')-#} [body] {#-PX, nl2'-#}"
+              using Htrue[of nl2'] by auto
+
+            have Ggood : "|#gs#| {#PX, (nb + nl2')#} ([body] @ [G SwhileC' [body]] @ c')" 
+              using HTiE[OF NB G1] by auto
+
+            have Almost :  "safe_for gs m' (nb + nl2')" using guardediD[OF Ggood M'] M'_cont
+              by auto
+
+            have Step : "sem_step_p gs m m'" using Inl
+              unfolding sem_step_p_eq
+              by auto
+      
+            have Step' : "sem_exec_c_p gs m 1 m'"
+              using sem_exec_c_p.intros(2)[OF Step sem_exec_c_p.intros(1)] by auto
+
+            have Conc' : "safe_for gs m (1 + nb + nl2')"
+              using safe_for_extend[OF Almost Step'] by auto
+
+            have Leq : "nl1 \<le> 1 + nb + nl2'" using Suc.prems by auto
+
+            show "safe_for gs m nl1"
+              using safe_for_weaken[OF Conc' Leq] by auto
+          next
+
+            case False
+
+            have M'_cont : "cont m' = Inl (c')"
+                using Hsyn H0 M' F_eq False Some' Hcontm  unfolding HF
+                by(cases m; auto simp add: cont_def sem_step_def imp_sem_l_gen_def imp_ctl_sem_def imp_sem_lifting_gen_def
+                  schem_lift_defs 
+                  merge_l_def fst_l_def snd_l_def prio_l_def triv_l_def option_l_def LNew_def
+                  get_cond_def
+                  split: md_prio.splits md_triv.splits option.splits)
+
+            have M'_full' : "PX (payload m') \<and> get_cond (payload m') = Some False"
+              using M' False Some' unfolding Suc.prems(1) Sm'
+              by auto
+
+            have Almost : "safe_for gs m' (Suc nl2')"
+              using guardediD[OF Suc.prems(1) M'_full' M'_cont] by auto
+
+            have Step : "sem_step_p gs m m'" using Inl
+              unfolding sem_step_p_eq
+              by auto
+
+            have Step' : "sem_exec_c_p gs m 1 m'"
+              using sem_exec_c_p.intros(2)[OF Step sem_exec_c_p.intros(1)] by auto
+
+            have Conc' : "safe_for gs m (1 + Suc (nl2'))"
+              using safe_for_extend[OF Almost Step'] by auto
+
+            have Leq : "nl1 \<le> 1 + Suc nl2'" using Suc.prems by auto
+
+            show "safe_for gs m nl1"
+              using safe_for_weaken[OF Conc' Leq] by auto
+          qed
+        qed
+      qed
+    qed
+  qed
+qed
+
+(* Using the soundness of our indexed Hoare triples, we can prove this rule in the normal
+ * Hoare abstraction.
+ * Note that because we could not prove completeness for the indexed triples,
+ * we still require an assumption on the body that talks about indices.
+ *)
+lemma HWhileC_idx :
+  assumes H0 : "gs = pcomps fs"
+  assumes HF : "f = imp_sem_l_gen lfts"
+  assumes Hpres : "sups_pres (set fs)"
+  assumes Hnemp : "g \<in> set fs"
+  assumes Hdom : "(f \<downharpoonleft> (set fs) SwhileC')"
+  assumes Hsyn : "lfts SwhileC' = SwhileC"
+  assumes PX_valid : "\<And> st.  PX st \<Longrightarrow> get_cond st \<noteq> None"
+  assumes Htrue : "|gs| {- PX-} [body] {- PX-}"
+  assumes NLs : "nl1 \<le> nl2"
+  shows "|gs| {-PX-} [G SwhileC' [body]] {- (\<lambda> st . PX st \<and> get_cond st = Some False)-}"
+proof(rule HT'_imp_HT; rule HT'I)
+  fix npre
+
+  have Htrue' : "\<And> nb2 . \<exists> nb1' . |#gs#| {#- PX, (nb1' + nb2) -#} [body] {#- PX, nb2 -#}"
+
+  show "\<exists>npost. |#gs#| {#-PX, npre-#} [G SwhileC' [body]] {#-(\<lambda>st. PX st \<and> get_cond st = Some False), npost-#}"
+
+
+end
