Language_Components/Seq/Seq_Hoare.thy
@@ -1,0 +1,190 @@
+theory Seq_Hoare imports 
+  Seq "../../Hoare/Hoare" "../../Composition/Composition" "../../Composition/Dominant"
+begin
+
+(* Hoare rule for Seq language *)
+
+
+(* TODO: this proof is currently rather nasty, as it
+ * involves unfolding a bunch of liftings. This is an opportunity to improve
+ * Auto_Lifter related automation.
+ *)
+
+(*
+ * Standard Seq Hoare rule. Included mostly for explanatory purposes since it is not able to
+ * make any guarantees in the context of Seq merged with other languages - it is "closed"
+ * in the sense of requiring a closed world (thus not especially useful).
+ * (See HSeq, below).
+ *)
+lemma HSeq_closed :
+  assumes H0 : "gs = seq_semx lfts"
+  assumes H1 : "lfts Sseq' = Sseq"
+  assumes H : "|gs| {- P1 -} cs {- P2 -}"
+  shows "|gs| {- P1 -} [G Sseq' cs] {- P2 -}"
+proof
+  fix c'
+  assume Safe : "|gs| {P2} c'"
+
+  have Guarded : "|gs| {P1} (cs @ c')"
+    using HTE[OF H Safe]
+    by auto
+
+  show "|gs| {P1} ([G Sseq' cs] @ c')"
+  proof
+    fix m :: "('a, 'b) control"
+    assume M : "P1 (payload m)"
+    assume CM : "cont m = Inl ([G Sseq' cs] @ c')"
+
+    show "(safe gs m)"
+    proof(cases "(sem_step gs m)")
+      case (Inr bad)
+
+      then have False using CM H0
+        by(auto simp add: sem_step_def)
+
+      then show ?thesis by auto
+    next
+      case (Inl m')
+
+(*TODO: make this less bad *)
+      have CM1 :  "cont m' = Inl (cs @ c')"
+        using Inl CM H0 H1
+        by(cases m; auto simp add: schem_lift_defs sem_step_def seq_semx_def seq_sem_l_gen_def seq_sem_def cont_def seq_sem_lifting_gen_def fst_l_def
+            prio_l_def option_l_def triv_l_def split: md_prio.splits option.splits md_triv.splits sum.splits)
+
+(*TODO: make this less bad *)
+      have M1_eq : "payload m' = payload m"
+        using Inl H0
+        by(cases m; auto simp add: schem_lift_defs sem_step_def seq_semx_def seq_sem_l_gen_def seq_sem_def cont_def seq_sem_lifting_gen_def fst_l_def
+            prio_l_def option_l_def triv_l_def split: md_prio.splits option.splits md_triv.splits list.split_asm)
+
+      have M1 : "P1 (payload m')" using M unfolding M1_eq by auto
+
+      have Step : "sem_step_p gs m m'"
+        using sem_step_sem_step_p[OF Inl] by auto
+
+      have Conc' : "safe gs m'" using guardedD[OF Guarded M1 CM1]
+        by auto
+
+      show "safe gs m"
+      proof
+        fix m''
+        assume XP : "sem_exec_p gs m m''"
+          
+        show "imm_safe gs m''" using XP unfolding sem_exec_p_def
+        proof(cases rule: rtranclp.cases)
+        case rtrancl_refl
+          then show ?thesis using imm_safeI_Step[OF Step] by auto
+        next
+          case RT : (rtrancl_into_rtrancl b)
+  
+          have Exc : "sem_exec_p gs m' m''" unfolding sem_exec_p_def using rtranclp_bisect1[OF sem_step_determ RT(1) Step RT(2)] by auto
+  
+          then show ?thesis using safeD[OF Conc' Exc] by auto
+        qed
+      qed
+    qed
+  qed
+qed
+
+(*
+ * More general version of HSeq that applies for any list fs of composed functions meeting
+ * certain conditions:
+ * - fs is nonempty
+ * - fs is dominated by sequence semantics for seq syntax
+ *)
+(* TODO: do we need the assumption that
+fs is nonempty? *)
+lemma HSeq_gen :
+  assumes H0 : "gs = pcomps fs "
+  (*assumes H1 : "seq_sem_l_gen lfts \<in> set fs" *)
+  assumes HF : "f = seq_sem_l_gen lfts"
+  assumes Hpres : "sups_pres (set fs)"
+  assumes Hnemp : "g \<in> set fs"
+  assumes Hdom : "(f \<downharpoonleft> (set fs) Sseq')"
+  assumes H2 : "lfts Sseq' = Sseq"
+  assumes H : "|gs| {- P1 -} cs {- P2 -}"
+  shows "|gs| {- P1 -} [G Sseq' cs] {- P2 -}"
+proof
+  fix c'
+  assume Guard : "|gs| {P2} c'"
+
+  have Guarded : "|gs| {P1} (cs @ c')"
+    using HTE[OF H Guard]
+    by auto
+
+  show "|gs| {P1} ([G Sseq' cs] @ c')"
+  proof
+    fix m :: "('a, 'b) control"
+    assume M : "P1 (payload m)"
+    assume CM : "cont m = Inl ([G Sseq' cs] @ c')"
+
+    show "(safe gs m)"
+    proof(cases "(sem_step gs m)")
+      case (Inr bad)
+
+      then have False using CM H0
+        by(auto simp add: sem_step_def)
+
+      then show ?thesis by auto
+    next
+      case (Inl m')
+
+      have F_eq : "sem_step f m = Inl m'"
+        using sym[OF dominant_pcomps[OF Hpres Hnemp Hdom]] CM Inl H0
+        by(simp add: sem_step_def)
+
+      have Fcont : "cont m' = Inl (cs @ c')"
+        using HF F_eq CM H2
+          (* TODO: better automation here *)
+        by(cases m; auto simp add: schem_lift_defs sem_step_def seq_sem_l_gen_def seq_semx_def seq_sem_def cont_def seq_sem_lifting_gen_def fst_l_def seq_sem_lifting'_def
+            prio_l_def option_l_def triv_l_def split: md_prio.splits option.splits md_triv.splits list.split_asm)
+
+
+      have Fstate : "payload m' = payload m"
+        using HF F_eq CM H2
+        by(cases m; auto simp add: schem_lift_defs sem_step_def seq_sem_l_gen_def seq_semx_def seq_sem_def cont_def seq_sem_lifting_gen_def fst_l_def seq_sem_lifting'_def
+            prio_l_def option_l_def triv_l_def split: md_prio.splits option.splits md_triv.splits list.split_asm)
+
+      hence M' :  "P1 (payload m')" using M unfolding Fstate by auto
+
+      have Safe' : "safe gs m'" using guardedD[OF Guarded M' Fcont] by auto
+
+      have Step : "sem_step_p gs m m'" using Inl
+        unfolding sem_step_p_eq
+        by auto
+
+      show "safe gs m" 
+      proof(rule safeI)
+        fix m''
+
+        assume Exec : "sem_exec_p gs m m''"
+        hence Exec' : "(sem_step_p gs)\<^sup>*\<^sup>* m m''"
+          unfolding sem_exec_p_def by auto
+
+        show "imm_safe gs m''" using Exec'
+        proof(cases rule: rtranclp.cases)
+          case rtrancl_refl
+          then show ?thesis 
+            using Inl 
+            unfolding imm_safe_def sem_step_p_eq
+            by(blast)
+        next
+          case (rtrancl_into_rtrancl b)
+
+          have Exec_final : "sem_exec_p gs m' m''"
+            using rtranclp_bisect1
+              [OF sem_step_determ rtrancl_into_rtrancl(1)
+                  Step rtrancl_into_rtrancl(2)]
+            unfolding sem_exec_p_def
+            by auto
+
+          show ?thesis using safeD[OF Safe' Exec_final] by auto
+        qed
+      qed
+    qed
+  qed
+qed
+
+
+end
