Language_Components/Utils.thy
@@ -1,0 +1,17 @@
+theory Utils
+  imports 
+  "../Syntax/Gensyn" "../Syntax/Gensyn_Descend" "../Mergeable/Mergeable" 
+  "../Mergeable/Mergeable_Instances"
+  "../Lifter/Lifter" "../Lifter/Lifter_Instances"
+begin
+
+(* Some miscellaneous code for use in developing language components
+   that didn't have a clear place elsewhere
+*)
+
+instantiation gensyn :: (Bogus) Bogus begin
+definition gensyn_bogus :
+"bogus = G bogus []"
+instance proof qed
+end
+end
